feat: more SAT API

src/Std/Sat/CNF/Basic.lean
@@ -1,7 +1,7 @@
 /-
 Copyright (c) 2024 Lean FRO, LLC. All rights reserved.
 Released under Apache 2.0 license as described in the file LICENSE.
-Authors: Kim Morrison
+Authors: Kim Morrison, Henrik Böving
 -/
 module
 
@@ -9,6 +9,8 @@ prelude
 public import Std.Sat.CNF.Literal
 public import Init.Data.Prod  -- shake: keep (proof instance elab'd in public scope, fix?)
 public import Init.Data.Array.Lemmas
+import Init.Data.Array.Bootstrap
+import Init.ByCases
 
 @[expose] public section
 
@@ -20,7 +22,9 @@ A clause in a CNF.
 
 The literal `(i, b)` is satisfied if the assignment to `i` agrees with `b`.
 -/
-abbrev CNF.Clause (α : Type u) : Type u := List (Literal α)
+structure CNF.Clause (α : Type u) where
+  literals : List (Literal α)
+  deriving DecidableEq, Inhabited
 
 /--
 A CNF formula.
@@ -32,14 +36,112 @@ structure CNF (α : Type u) where
 
 namespace CNF
 
+namespace Clause
+
+@[inline]
+def empty : Clause α := ⟨[]⟩
+
+@[inline]
+def add (c : Clause α) (atom : α) (pol : Bool) : Clause α :=
+  { c with literals := (atom, pol) :: c.literals }
+
+@[simp]
+theorem add_ne_empty (c : Clause α) (atom : α) (pol : Bool) : c.add atom pol ≠ empty := by
+  simp [empty, add]
+
 /--
 Evaluating a `Clause` with respect to an assignment `a`.
 -/
-def Clause.eval (a : α → Bool) (c : Clause α) : Bool := c.any fun (i, n) => a i == n
+def eval (a : α → Bool) (c : Clause α) : Bool := c.literals.any fun (i, n) => a i == n
 
-@[simp] theorem Clause.eval_nil (a : α → Bool) : Clause.eval a [] = false := rfl
-@[simp] theorem Clause.eval_cons (a : α → Bool) :
-    Clause.eval a (i :: c) = (a i.1 == i.2 || Clause.eval a c) := rfl
+@[simp] theorem eval_empty (a : α → Bool) : Clause.eval a .empty = false := rfl
+@[simp] theorem eval_add (a : α → Bool) :
+    Clause.eval a (c.add atom pol) = (a atom == pol || Clause.eval a c) := rfl
+
+instance : Membership (Literal α) (Clause α) where
+  mem clause lit := lit ∈ clause.literals
+
+instance [Monad m] : ForIn' m (Clause α) (Literal α) inferInstance where
+  forIn' clause b f := forIn' clause.literals b f
+
+theorem mem_literals_iff {c : Clause α} {l : Literal α} : l ∈ c.literals ↔ l ∈ c := Iff.rfl
+
+@[simp]
+theorem not_mem_empty {l : Literal α} : l ∉ (empty : Clause α) := by
+  simp [← mem_literals_iff, empty]
+
+@[simp]
+theorem mem_add {c : Clause α} {l1 : Literal α} : l1 ∈ c.add atom pol ↔ l1 = (atom, pol) ∨ l1 ∈ c := by
+  simp [← mem_literals_iff, add]
+
+theorem forIn'_eq_forIn'_literals [Monad m] {c : Clause α} {init : β}
+    {f : (l : Literal α) → l ∈ c → β → m (ForInStep β)} :
+    forIn' c init f = forIn' c.literals init (fun l h b => f l (mem_literals_iff.mp h) b) :=
+  rfl
+
+def Sat (a : α → Bool) (f : Clause α) : Prop := eval a f = true
+def Unsat (f : Clause α) : Prop := ∀ a, eval a f = false
+
+theorem sat_def (a : α → Bool) (f : Clause α) : Sat a f ↔ (eval a f = true) := by rfl
+theorem unsat_def (f : Clause α) : Unsat f ↔ (∀ a, eval a f = false) := by rfl
+
+@[simp] theorem unsat_empty : Unsat (.empty : Clause α) := by
+  simp [unsat_def]
+
+@[simp] theorem not_sat_empty {a : α → Bool} : ¬ Sat a (.empty : Clause α) := by
+  simp [sat_def]
+
+@[simp] theorem sat_add {a : α → Bool} {c : Clause α} :
+    Sat a (c.add atom pol) ↔ a atom = pol ∨ Sat a c := by
+  simp [sat_def]
+
+theorem unsat_iff_not_sat {c : Clause α} : Unsat c ↔ ∀ a, ¬Sat a c := by
+  rw [unsat_def]
+  constructor
+  · intro h1 a h2
+    rw [sat_def] at h2
+    simp_all
+  · intro h1 a
+    specialize h1 a
+    rw [sat_def] at h1
+    simp_all
+
+theorem sat_iff_exists_mem_eq {c : Clause α} :
+    Sat a c ↔ (∃ lit ∈ c, a lit.1 = lit.2) := by
+  simp [sat_def, Membership.mem, eval]
+
+theorem sat_of_mem_of_eq {c : Clause α} {lit : Literal α} (h1 : lit ∈ c) (h2 : a lit.1 = lit.2) :
+    Sat a c :=
+  sat_iff_exists_mem_eq.mpr ⟨lit, h1, h2⟩
+
+theorem not_sat_iff_forall_mem_ne {c : Clause α} :
+    (¬ Sat a c) ↔ (∀ lit ∈ c, a lit.1 ≠ lit.2) := by
+  rw [sat_iff_exists_mem_eq]
+  simp only [not_exists, not_and, ne_eq]
+
+theorem sat_of_mem_of_mem_neg {c : Clause α} {atom : α} (h1 : (atom, pol) ∈ c)
+    (h2 : (atom, !pol) ∈ c) : ∀ a, Sat a c := by
+  intro a
+  rw [sat_iff_exists_mem_eq]
+  by_cases h3 : a atom = pol
+  · exists (atom, pol)
+  · exists (atom, !pol)
+    cases pol <;> simp_all
+
+open Classical in
+theorem unsat_iff_eq_empty {c : Clause α} : Unsat c ↔ c = .empty := by
+  constructor
+  · intro h
+    rcases c with ⟨_ | ⟨lit, lits⟩⟩
+    · rfl
+    · exfalso
+      have hmem : lit ∈ (⟨lit :: lits⟩ : Clause α) := by simp [← mem_literals_iff]
+      have hsat := sat_of_mem_of_eq (a := fun v => if v = lit.1 then lit.2 else true) hmem (by simp)
+      exact unsat_iff_not_sat.mp h _ hsat
+  · rintro rfl
+    exact unsat_empty
+
+end Clause
 
 /--
 Evaluating a `CNF` formula with respect to an assignment `a`.
@@ -76,53 +178,82 @@ def Unsat (f : CNF α) : Prop := ∀ a, eval a f = false
 theorem sat_def (a : α → Bool) (f : CNF α) : Sat a f ↔ (eval a f = true) := by rfl
 theorem unsat_def (f : CNF α) : Unsat f ↔ (∀ a, eval a f = false) := by rfl
 
-
 @[simp] theorem not_unsat_empty : ¬Unsat (.empty : CNF α) :=
   fun h => by simp [unsat_def] at h
 
 @[simp] theorem sat_empty {assign : α → Bool} : Sat assign (.empty : CNF α) := by
   simp [sat_def]
 
-@[simp] theorem unsat_add_nil {g : CNF α} : Unsat (g.add []) := by
+@[simp]
+theorem sat_add {assign : α → Bool} {f : CNF α} :
+    Sat assign (f.add c : CNF α) ↔ (Clause.Sat assign c ∧ Sat assign f) := by
+  simp [sat_def, Clause.sat_def]
+
+@[simp]
+theorem sat_append {assign : α → Bool} :
+    Sat assign (f1 ++ f2 : CNF α) ↔ (Sat assign f1 ∧ Sat assign f2) := by
+  simp [sat_def]
+
+@[simp] theorem unsat_add_empty {g : CNF α} : Unsat (g.add .empty) := by
   simp [unsat_def]
+
+theorem unsat_iff_not_sat {f : CNF α} : Unsat f ↔ ∀ a, ¬Sat a f := by
+  rw [unsat_def]
+  constructor
+  · intro h1 a h2
+    rw [sat_def] at h2
+    simp_all
+  · intro h1 a
+    specialize h1 a
+    rw [sat_def] at h1
+    simp_all
 
 namespace Clause
 
 /--
 Variable `v` occurs in `Clause` `c`.
 -/
-def Mem (v : α) (c : Clause α) : Prop := (v, false) ∈ c ∨ (v, true) ∈ c
+def VarMem (v : α) (c : Clause α) : Prop := (v, false) ∈ c.literals ∨ (v, true) ∈ c.literals
 
-instance {v : α} {c : Clause α} [DecidableEq α] : Decidable (Mem v c) :=
+instance {v : α} {c : Clause α} [DecidableEq α] : Decidable (VarMem v c) :=
   inferInstanceAs <| Decidable (_ ∨ _)
 
-@[simp] theorem not_mem_nil {v : α} : ¬Mem v ([] : Clause α) := by simp [Mem]
-@[simp] theorem mem_cons {v : α} : Mem v (l :: c : Clause α) ↔ (v = l.1 ∨ Mem v c) := by
-  rcases l with ⟨b, (_|_)⟩
-  · simp [Mem, or_assoc]
-  · simp [Mem]
-    rw [or_left_comm]
+@[simp] theorem not_VarMem_empty {v : α} : ¬VarMem v .empty := by simp [VarMem, empty]
 
-theorem mem_of (h : (v, p) ∈ c) : Mem v c := by
-  cases p
-  · left; exact h
-  · right; exact h
+theorem VarMem_add_self {c : Clause α} : VarMem atom (c.add atom pol) := by
+  cases pol <;> simp [VarMem, add]
 
-theorem eval_congr (a1 a2 : α → Bool) (c : Clause α) (hw : ∀ i, Mem i c → a1 i = a2 i) :
+theorem VarMem_add_ne_self {c : Clause α} {atom1 atom2 : α} (h : atom1 ≠ atom2) :
+    VarMem atom1 (c.add atom2 pol) ↔ VarMem atom1 c := by
+  simp [VarMem, add, h]
+
+@[simp] theorem VarMem_add {v : α} : VarMem v (c.add atom pol) ↔ (v = atom ∨ VarMem v c) := by
+  by_cases h : v = atom
+  · simp [VarMem_add_self, h]
+  · simp [VarMem_add_ne_self, h]
+
+@[elab_as_elim]
+theorem induct {motive : Clause α → Prop} (empty : motive .empty)
+    (add : (c : Clause α) → (atom : α) → (pol : Bool) → motive c → motive (c.add atom pol))
+    (c : Clause α) : motive c := by
+  rcases c with ⟨ls⟩
+  induction ls with
+  | nil => exact empty
+  | cons l ls ih =>
+    specialize add ⟨ls⟩ l.1 l.2 ih
+    exact add
+
+theorem eval_congr (a1 a2 : α → Bool) (c : Clause α) (hw : ∀ i, VarMem i c → a1 i = a2 i) :
     eval a1 c = eval a2 c := by
-  induction c
-  case nil => rfl
-  case cons i c ih =>
-    simp only [eval_cons]
+  induction c using induct with
+  | empty => simp
+  | add c atom pol ih =>
+    simp
     rw [ih, hw]
-    · rcases i with ⟨b, (_|_)⟩ <;> simp [Mem]
-    · intro j h
+    · simp
+    · intro i hm
       apply hw
-      rcases h with h | h
-      · left
-        apply List.mem_cons_of_mem _ h
-      · right
-        apply List.mem_cons_of_mem _ h
+      simp [hm]
 
 end Clause
 
@@ -137,18 +268,71 @@ instance : Membership (Clause α) (CNF α) where
 instance {c : Clause α} {f : CNF α} [DecidableEq α] : Decidable (c ∈ f) :=
     inferInstanceAs <| Decidable (c ∈ f.clauses)
 
+theorem Internal.mem_iff {f : CNF α} : c ∈ f ↔ c ∈ f.clauses := by
+  rfl
+
+theorem Internal.clauses_append {f1 f2 : CNF α} : (f1 ++ f2).clauses = f1.clauses ++ f2.clauses := rfl
+
+@[simp]
+theorem not_mem_empty {c : Clause α} : c ∉ (empty : CNF α) := by
+  simp [Internal.mem_iff, empty]
+
+@[simp]
+theorem mem_add {f : CNF α} {c1 c2 : Clause α} : c1 ∈ f.add c2 ↔ c1 = c2 ∨ c1 ∈ f := by
+  simp [Internal.mem_iff, add, or_comm]
+
+@[simp]
+theorem mem_append {f1 f2 : CNF α} {c : Clause α} : c ∈ (f1 ++ f2) ↔ c ∈ f1 ∨ c ∈ f2 := by
+  simp [Internal.mem_iff, Internal.clauses_append]
+
+theorem sat_iff_all_mem_sat {f : CNF α} {a : α → Bool} : Sat a f ↔ ∀ c ∈ f, Clause.Sat a c := by
+  simp only [sat_def, Clause.sat_def, eval]
+  rw [Array.all_eq_true_iff_forall_mem]
+  rfl
+
+theorem sat_of_mem {f : CNF α} (h1 : Sat a f) (h2 : c ∈ f) : Clause.Sat a c :=
+  sat_iff_all_mem_sat.mp h1 c h2
+
+theorem not_sat_iff_exists_mem_not_sat {f : CNF α} :
+    (¬Sat a f) ↔ (∃ c ∈ f, ¬Clause.Sat a c) := by
+  simp only [sat_def, Clause.sat_def, eval, Bool.not_eq_true, Array.all_eq_false',
+    Internal.mem_iff]
+
+theorem unsat_of_mem_unsat {f : CNF α} (h1 : c ∈ f) (h2 : Clause.Unsat c) : Unsat f := by
+  rw [unsat_iff_not_sat]
+  intro a hsat
+  exact Clause.unsat_iff_not_sat.mp h2 a (sat_of_mem hsat h1)
+
+theorem unsat_add_of_clause_unsat {f : CNF α} (h : Clause.Unsat c) : Unsat (f.add c) :=
+  unsat_of_mem_unsat (by simp) h
+
+theorem unsat_add_of_unsat {f : CNF α} (h : Unsat f) : Unsat (f.add c) := by
+  rw [unsat_iff_not_sat] at h ⊢
+  intro a hsat
+  exact h a (sat_add.mp hsat).right
+
+theorem unsat_append_left {f1 f2 : CNF α} (h : Unsat f1) : Unsat (f1 ++ f2) := by
+  rw [unsat_iff_not_sat] at h ⊢
+  intro a hsat
+  exact h a (sat_append.mp hsat).left
+
+theorem unsat_append_right {f1 f2 : CNF α} (h : Unsat f2) : Unsat (f1 ++ f2) := by
+  rw [unsat_iff_not_sat] at h ⊢
+  intro a hsat
+  exact h a (sat_append.mp hsat).right
+
 /--
 Variable `v` occurs in `CNF` formula `f`.
 -/
-def VarMem (v : α) (f : CNF α) : Prop := ∃ c, c ∈ f.clauses ∧ c.Mem v
+def VarMem (v : α) (f : CNF α) : Prop := ∃ c, c ∈ f.clauses ∧ c.VarMem v
 
 instance {v : α} {f : CNF α} [DecidableEq α] : Decidable (VarMem v f) :=
   inferInstanceAs <| Decidable (∃ _, _)
 
 theorem Internal.any_not_isEmpty_iff_exists_mem {f : CNF α} :
-    (f.clauses.any fun c => !List.isEmpty c) = true ↔ ∃ v, VarMem v f := by
+    (f.clauses.any fun c => !List.isEmpty c.literals) = true ↔ ∃ v, VarMem v f := by
   simp only [Array.any_eq_true, Bool.not_eq_true', List.isEmpty_eq_false_iff_exists_mem, VarMem,
-    Clause.Mem]
+    Clause.VarMem]
   constructor
   · intro h
     rcases h with ⟨idx, ⟨hclause1, hclause2⟩⟩
@@ -173,12 +357,12 @@ theorem Internal.any_not_isEmpty_iff_exists_mem {f : CNF α} :
 
 @[no_expose]
 instance {f : CNF α} [DecidableEq α] : Decidable (∃ v, VarMem v f) :=
-  decidable_of_iff (f.clauses.any fun c => !c.isEmpty) Internal.any_not_isEmpty_iff_exists_mem
+  decidable_of_iff (f.clauses.any fun c => !c.literals.isEmpty) Internal.any_not_isEmpty_iff_exists_mem
 
 theorem not_VarMem_empty {v : α} : ¬VarMem v (.empty : CNF α) := by simp [VarMem, empty]
 
 @[local simp] theorem VarMem_add {v : α} {c} {f : CNF α} :
-    VarMem v (f.add c : CNF α) ↔ (Clause.Mem v c ∨ VarMem v f) := by
+    VarMem v (f.add c : CNF α) ↔ (Clause.VarMem v c ∨ VarMem v f) := by
   simp only [VarMem, add, Array.mem_push]
   constructor
   · intro h
@@ -193,17 +377,26 @@ theorem not_VarMem_empty {v : α} : ¬VarMem v (.empty : CNF α) := by simp [Var
     · exists c
       simp [hc1, hc2]
 
-theorem VarMem_of (h : c ∈ f) (w : Clause.Mem v c) : VarMem v f := by
+theorem VarMem_of (h : c ∈ f) (w : Clause.VarMem v c) : VarMem v f := by
   apply Exists.intro c
   constructor <;> assumption
 
-theorem Internal.mem_iff {f : CNF α} : c ∈ f ↔ c ∈ f.clauses := by
-  rfl
-
-theorem Internal.clauses_append {f1 f2 : CNF α} : (f1 ++ f2).clauses = f1.clauses ++ f2.clauses := rfl
-
 theorem Internal.ext_iff {f1 f2 : CNF α} : f1 = f2 ↔ f1.clauses = f2.clauses := by
   cases f1; cases f2; simp
+
+@[simp]
+theorem append_empty {f : CNF α} : f ++ (empty : CNF α) = f := by
+  rw [Internal.ext_iff, Internal.clauses_append]
+  simp [empty]
+
+@[simp]
+theorem empty_append {f : CNF α} : (empty : CNF α) ++ f = f := by
+  rw [Internal.ext_iff, Internal.clauses_append]
+  simp [empty]
+
+@[simp]
+theorem append_assoc {f1 f2 f3 : CNF α} : (f1 ++ f2) ++ f3 = f1 ++ (f2 ++ f3) := by
+  simp [Internal.ext_iff, Internal.clauses_append, Array.append_assoc]
 
 @[simp]
 theorem emptyWithCapacity_eq_empty (n : Nat) :
