src/Std/Sat/CNF.lean
@@ -11,3 +11,5 @@ public import Std.Sat.CNF.Literal
 public import Std.Sat.CNF.Relabel
 public import Std.Sat.CNF.RelabelFin
 public import Std.Sat.CNF.Dimacs
+public import Std.Sat.CNF.Entails
+public import Std.Sat.CNF.Unit
